Major improvements
- The semantics was updated to be compliant with a more recent version of Solidity (v0.8.25).
- In addition to external functions it now also supports internal functions.
- In addition to the verification of invariants, it now also supports the verification of (multiple) pre/post-conditions for functions.
- Type consistency is added as pre-condition for functions.

Casino.thy
@@ -1,22 +1,12 @@
-theory Casino
-  imports Solidity_Main
+theory Casino 
+  imports Solidity_Main "HOL-Eisbach.Eisbach" "HOL-Eisbach.Eisbach_Tools"
 begin
 
-lemma sym[wpdrules]:
-  assumes "rvalue.Value v = y"
-    shows "y = rvalue.Value v"
-  using assms by simp
-
-lemma sym2[wpdrules]:
-  assumes "sdata.Value v = y"
-    shows "y = sdata.Value v"
-  using assms by simp
-
 section \<open>Casino Contract\<close>
-
 text \<open>
   In the following we verify the Casino contract from the VerifyThis Long-Term Challenge:
-  \<^url>\<open>https://verifythis.github.io/02casino/\<close>.
+  \<^url>\<open>https://verifythis.github.io/02casino/\<close>
+  \<^url>\<open>https://verifythis.github.io/ltc/02casino/\<close>.
 \<close>
 
 subsection \<open>Specification\<close>
@@ -29,18 +19,43 @@ text \<open>
   Method modifiers are formalized as abbreviations.
   They need to be formalized in the Solidity context to provide access to various contextual information.
 \<close>
+abbreviation "state \<equiv> STR ''state''"
+abbreviation "operator \<equiv> STR ''operator''"
+abbreviation "player \<equiv> STR ''player''"
+abbreviation "pot \<equiv> STR ''pot''"
+abbreviation "hashedNumber \<equiv> STR ''hashedNumber''"
+abbreviation "bet \<equiv> STR ''bet''"
+abbreviation "guess \<equiv> STR ''guess''"
+abbreviation "hashNum \<equiv> STR ''hashNum''"
+abbreviation "secret \<equiv> STR ''secret''"
+abbreviation "bet_old \<equiv> STR ''bet_old''"
+abbreviation "secretNumber \<equiv> STR ''secretNumber''"
+abbreviation "amount \<equiv> STR ''amount''"
+
+
+abbreviation "IDLE \<equiv> 0"
+abbreviation "GAME_AVAILABLE \<equiv> 1"
+abbreviation "BET_PLACED \<equiv> 2"
+abbreviation "HEADS \<equiv> 0"
+abbreviation "TAILS \<equiv> 1"
+abbreviation "CoinT \<equiv> SType.TValue TSint"
+abbreviation "StateT \<equiv> SType.TValue TSint"
+abbreviation "AddressT \<equiv> SType.TValue TAddress"
+abbreviation "IntT \<equiv> SType.TValue TSint"
+abbreviation "Bytes32T \<equiv> SType.TValue (TBytes 32)"
+
 
 context Solidity
 begin
 
 abbreviation byOperator::"(unit, ex, 'a state) state_monad" where
-  "byOperator \<equiv> assert Err (\<lambda>s. sdata.Value (valtype.Address msg_sender) = state.Storage s this (STR ''operator''))"
+  "byOperator \<equiv> assert Err (\<lambda>s. storage_data.Value (valtype.Address msg_sender) = state.Storage s this operator)"
 
 abbreviation inState:: "'a valtype \<Rightarrow> (unit, ex, 'a state) state_monad" where
-  "inState state \<equiv> assert Err (\<lambda>s. state.Storage s this (STR ''state'') = sdata.Value state)"
+  "inState st \<equiv> assert Err (\<lambda>s. state.Storage s this state = storage_data.Value st)"
 
 abbreviation noActiveBet::"(unit, ex, ('a, 'b) state_scheme) state_monad" where
-  "noActiveBet \<equiv> assert Err (\<lambda>s. state.Storage s this (STR ''state'') \<noteq> sdata.Value (Sint 2))"
+  "noActiveBet \<equiv> assert Err (\<lambda>s. state.Storage s this state \<noteq> storage_data.Value (Uint 2))"
 
 end
 
@@ -51,121 +66,92 @@ text \<open>
   \<^item> A constructor
   \<^item> A sequence of methods
 \<close>
-ML \<open>
-  val pretty_term = Syntax.pretty_term
-
-  val pwriteln = Pretty.writeln
-
-  fun pretty_terms ctxt trms =
-    Pretty.block (Pretty.commas (map (pretty_term ctxt) trms))
-
-  fun pretty_typ ctxt ty = Syntax.pretty_typ ctxt ty
-
-  fun pretty_typs ctxt tys =
-    Pretty.block (Pretty.commas (map (pretty_typ ctxt) tys))
-
-  fun pretty_thm ctxt thm =
-    pretty_term ctxt (Thm.prop_of thm)
-\<close>
 
 contract Casino
-  for "STR ''state''": "sdata.Value sint"
-  and "STR ''operator''": "sdata.Value address"
-  and "STR ''player''": "sdata.Value address"
-  and "STR ''pot''": "sdata.Value sint"
-  and "STR ''hashedNumber''": "sdata.Value bytes"
-  and "STR ''bet''": "sdata.Value sint"
-  and "STR ''guess''": "sdata.Value sint"
+  for state: StateT
+  and operator: AddressT
+  and player: AddressT
+  and pot: IntT
+  and hashedNumber: Bytes32T
+  and bet: IntT
+  and guess: CoinT
 
-constructor
+constructor payable
 where
-  "skip_monad"
+  "\<langle>skip\<rangle>"
 
-cmethod createGame
-  param "STR ''hashNum''": "Bytes hashNum"
+cfunction createGame external payable
+  param hashNum: "SType.TValue (TBytes 32)"
 where
   "do {
     byOperator;
-    inState (valtype.Sint 0);
-    assign_storage_monad (STR ''hashedNumber'') [] (stackLookup (STR ''hashNum'') []);
-    assign_storage_monad (STR ''state'') [] (sint_monad 1)
+    inState (valtype.Uint 0);
+    hashedNumber [] ::=\<^sub>s hashNum ~ [];
+    state [] ::=\<^sub>s \<langle>sint\<rangle> 1
    }",
 
-cmethod placeBet
-  param "STR ''guess''": "Sint guess"
+cfunction placeBet external payable
+  param guess: "SType.TValue TSint"
 where
   "do {
-    inState (valtype.Sint 1);
-    assert_monad (not_monad (equals_monad sender_monad (storeLookup (STR ''operator'') [])));
-    assert_monad (not_monad (equals_monad value_monad (storeLookup (STR ''pot'') [])));
-    assign_storage_monad (STR ''state'') [] (sint_monad 2);
-    assign_storage_monad (STR ''player'') [] sender_monad;
-    assign_storage_monad (STR ''bet'') [] value_monad;
-    assign_storage_monad (STR ''guess'') [] (stackLookup (STR ''guess'') [])
+    inState (valtype.Uint 1);
+    \<langle>assert\<rangle> (\<langle>\<not>\<rangle> (\<langle>sender\<rangle> \<langle>=\<rangle> operator ~\<^sub>s []));
+    \<langle>assert\<rangle> (\<langle>value\<rangle> \<langle><\<rangle> (pot  ~\<^sub>s []) \<langle>\<or>\<rangle> \<langle>value\<rangle> \<langle>=\<rangle> (pot ~\<^sub>s []));
+    state [] ::=\<^sub>s \<langle>sint\<rangle> 2;
+    player [] ::=\<^sub>s \<langle>sender\<rangle>;
+    bet [] ::=\<^sub>s \<langle>value\<rangle>;
+    guess [] ::=\<^sub>s guess ~ []
   }",
 
-cmethod decideBet
-  param "STR ''secretNumber''": "Sint secretNumber"
-where
-  "do {
-    byOperator;
-    inState (valtype.Sint 2);
-    assert_monad (equals_monad (storeLookup (STR ''hashedNumber'') []) (keccak256_monad (stackLookup (STR ''secretNumber'') [])));
-    init (STR ''secret'') (sint :: 'a valtype);
-    assign_stack_monad (STR ''secret'') [] (cond_monad (equals_monad (mod_monad (stackLookup (STR ''secretNumber'') []) (sint_monad 2)) (sint_monad 0)) (bool_monad True) (bool_monad False));
-    cond_monad (equals_monad (stackLookup (STR ''secret'') []) (storeLookup (STR ''guess'') []))
-      (do {
-        assign_stack_monad (STR ''pot'') [] (minus_monad (storeLookup (STR ''pot'') []) (storeLookup (STR ''bet'') []));
-        transfer_monad (storeLookup (STR ''player'') []) (mult_monad (storeLookup (STR ''bet'') []) (sint_monad 2));
-        assign_stack_monad (STR ''bet'') [] (sint_monad 0)
-       })
-      (do {
-        assign_stack_monad (STR ''pot'') [] (plus_monad (storeLookup (STR ''pot'') []) (storeLookup (STR ''bet'') []));
-        assign_stack_monad (STR ''bet'') [] (sint_monad 0)
-       });
-    assign_storage_monad (STR ''state'') [] (sint_monad 0)
-  }",
-
-cmethod addToPot
+cfunction decideBet external payable
+  param secretNumber: IntT
 where
   "do {
     byOperator;
-    assign_storage_monad (STR ''pot'') [] (plus_monad_safe (storeLookup (STR ''pot'') []) value_monad)
+    inState (Uint BET_PLACED);
+    \<langle>assert\<rangle> (hashedNumber ~\<^sub>s [] \<langle>=\<rangle> (\<langle>keccak256\<rangle> (secretNumber ~ [])));
+    decl TSint secret;
+    secret [] ::= IF ((secretNumber ~ []) \<langle>%\<rangle> \<langle>sint\<rangle> 2) \<langle>=\<rangle> (\<langle>sint\<rangle> 0) THEN \<langle>sint\<rangle> HEADS ELSE \<langle>sint\<rangle> TAILS;
+    IF (secret ~ []) \<langle>=\<rangle> (guess ~\<^sub>s []) THEN
+      do {
+        pot [] ::=\<^sub>s ((pot ~\<^sub>s []) \<langle>-\<rangle> (bet ~\<^sub>s []));
+        bet [] ::=\<^sub>s \<langle>sint\<rangle> 0;
+        \<langle>transfer\<rangle> (player ~\<^sub>s []) ((bet ~\<^sub>s []) \<langle>*\<rangle> (\<langle>sint\<rangle> 2))
+      }
+    ELSE
+      do {
+        pot [] ::=\<^sub>s pot ~\<^sub>s [] \<langle>+\<rangle> bet ~\<^sub>s [];
+        bet [] ::=\<^sub>s \<langle>sint\<rangle> 0
+      };
+    state [] ::=\<^sub>s \<langle>sint\<rangle> IDLE
   }",
 
-cmethod removeFromPot
-  param "STR ''amount''": "Sint amount"
+cfunction addToPot external payable
+where
+  "do {
+    byOperator;
+    pot [] ::=\<^sub>s pot ~\<^sub>s [] \<langle>+\<rangle> \<langle>value\<rangle>
+  }",
+
+cfunction removeFromPot external payable
+  param amount: "SType.TValue TSint"
 where
   "do {
     byOperator;
     noActiveBet;
-    assign_storage_monad (STR ''pot'') [] (minus_monad_safe (storeLookup (STR ''pot'') []) (stackLookup (STR ''amount'') []));
-    transfer_monad (storeLookup (STR ''operator'') []) (stackLookup (STR ''amount'') [])
+    pot [] ::=\<^sub>s ((pot ~\<^sub>s []) \<langle>-\<rangle> (amount ~ []));
+    \<langle>transfer\<rangle> (operator ~\<^sub>s []) (amount ~ [])
   }"
 
-text (in Solidity) \<open>
-  The contract command creates definitions for the constructor and each method:
-  \<^item> @{thm Casino.Solidity.casino_constructor_def [no_vars]}
-  \<^item> @{thm Casino.Solidity.createGame_def [no_vars]}
-  \<^item> ...
+thm casino.addToPot_def
 
-  In addition it creates and proves monotonicity lemmas for the partial\_function package for each method:
-  \<^item> @{thm createGame_def_mono [no_vars]}
-
-  It also creates a datatype for the contract:
-  \<^item> @{typ "'a Solidity.casino"}
-  with constructors for each method:
-  \<^item> @{term Casino.Solidity.casino.CreateGame_m}
-
-  Finally it creates a recursive definition using the partial\_function package in mode sm:
-  \<^item> @{term Casino.Solidity.call}
-  \<^item> @{thm Casino.Solidity.call.simps [no_vars]}
-  
-  The proof obligations are discharged using the previously generated monotonicity lemmas.
-
-  The partial\_function package provides us with an induction rule:
-  @{thm Casino.Solidity.call.raw_induct [no_vars]}
-\<close>
+invariant pot_balance sb where
+    "(fst sb state = storage_data.Value (Uint BET_PLACED)
+      \<longrightarrow> snd sb \<ge> unat (valtype.uint (storage_data.vt (fst sb pot))) + unat (valtype.uint (storage_data.vt (fst sb bet)))
+        \<and> valtype.uint (storage_data.vt (fst sb bet)) \<le> valtype.uint (storage_data.vt (fst sb pot))) \<and>
+    (fst sb state \<noteq> storage_data.Value (Uint BET_PLACED)
+      \<longrightarrow> snd sb \<ge> unat (valtype.uint (storage_data.vt (fst sb pot))))"
+  for "casino"
 
 section \<open>Verifying an Invariant\<close>
 
@@ -175,173 +161,327 @@ text \<open>
   Note that an invariant is formalized as a predicate over the contracts state and balance.
 \<close>
 
-definition pot_balance:: "(id \<Rightarrow> 'a::address sdata) \<times> nat \<Rightarrow> bool"
-  where "pot_balance sb \<equiv>
-          (\<exists>x. (fst sb) (STR ''state'') = sdata.Value (Sint x)) \<and>
-          (\<exists>x. (fst sb) (STR ''operator'') = sdata.Value (Address x)) \<and>
-          (\<exists>x. (fst sb) (STR ''player'') = sdata.Value (Address x)) \<and>
-          (\<exists>x. (fst sb) (STR ''pot'') = sdata.Value (Sint x)) \<and>
-          (\<exists>x. (fst sb) (STR ''hashedNumber'') = sdata.Value (Bytes x)) \<and>
-          (\<exists>x. (fst sb) (STR ''bet'') = sdata.Value (Sint x)) \<and>
-          (\<exists>x. (fst sb) (STR ''guess'') = sdata.Value (Sint x)) \<and>
-          (\<forall>x. (fst sb) (STR ''pot'') = sdata.Value (Sint (x)) \<longrightarrow> (snd sb) \<ge> unat x)"
-
-text \<open>We need to create introduction and elimination rules for the invariant and add it to the wprule and wperule lists.\<close>
-
-lemma pot_balanceI[wprule]:
-  assumes "s (STR ''state'') = sdata.Value (Sint state)"
-     and  "s (STR ''operator'') = sdata.Value (Address operator)"
-     and  "s (STR ''player'') = sdata.Value (Address player)"
-     and  "s (STR ''pot'') = sdata.Value (Sint pot)"
-     and  "s (STR ''hashedNumber'') = sdata.Value (Bytes hashedNumber)"
-     and  "s (STR ''bet'') = sdata.Value (Sint bet)"
-     and  "s (STR ''guess'') = sdata.Value (Sint guess)"
-     and  "\<And>x. s (STR ''pot'') = sdata.Value (Sint (x)) \<Longrightarrow> b \<ge> unat x"
-  shows "pot_balance (s, b)"
-  unfolding pot_balance_def using assms by simp
-
-lemma pot_balanceE[wperule]:
-  assumes "pot_balance (s, b)"
-  obtains state operator player pot hashedNumber bet guess
-  where "s (STR ''state'') = sdata.Value (Sint state)"
-    and "s (STR ''operator'') = sdata.Value (Address operator)"
-    and "s (STR ''player'') = sdata.Value (Address player)"
-    and "s (STR ''pot'') = sdata.Value (Sint pot)"
-    and "s (STR ''hashedNumber'') = sdata.Value (Bytes hashedNumber)"
-    and "s (STR ''bet'') = sdata.Value (Sint bet)"
-    and "s (STR ''guess'') = sdata.Value (Sint guess)"
-    and "\<And>x. s (STR ''pot'') = sdata.Value (Sint (x)) \<Longrightarrow> b \<ge> unat x"
-  using assms unfolding pot_balance_def by auto
+text \<open>We need to create introduction and elimination rules for the invariant and add it to the wprules and wperule lists.\<close>
 
 text \<open>
   Now we can start verifying the invariant.
   To this end our package provides a keyword invariant which takes a property as parameter and generates proof obligations.
 \<close>
 
-context Solidity
+context casino
 begin
 
-lemma constructor_casino:
-  assumes "effect casino_constructor s r"
-    shows "local.inv r (inv_state pot_balance) (inv_state pot_balance)"
-  using assms
-  apply (erule_tac inv_wp)
-  unfolding casino_constructor_def inv_state_def
-  by (vcg | auto)+
+lemma sym2:
+  assumes "storage_data.Value v = state.Storage s this x"
+    shows "state.Storage s this x = storage_data.Value v"
+  using assms by simp
 
-lemma createGame:
-    fixes call:: "'a casino \<Rightarrow> (unit, ex, ('a::address) state) state_monad"
-  assumes "effect (createGame callx x) s r"
-      and "inv_state pot_balance s" 
-    shows "inv r (inv_state pot_balance) (inv_state pot_balance)"
+lemma kdequals_true_dest[wpdrules]:
+  assumes "kdequals a b = Some (rvalue.Value (Bool True))"
+  shows "a = b"
   using assms
-  apply (erule_tac inv_wp)
-  unfolding createGame_def inv_state_def
-  by (vcg | auto)+
+  apply (cases a;simp add: kdequals_def)
+  apply (cases b;simp add: kdequals_def)
+  by (case_tac x4;case_tac x4a;simp add: kdequals_def split: if_split_asm)
 
-lemma placeBet:
-    fixes call:: "'a casino \<Rightarrow> 'a expression_monad"
-    assumes "effect (placeBet call x) s r"
-        and "inv_state pot_balance s" 
-    shows "inv r (inv_state pot_balance) (inv_state pot_balance)"
-  using assms
-  apply (erule_tac inv_wp)
-  unfolding placeBet_def inv_state_def
-  by (vcg | auto)+
 
-lemma decideBet:
-    fixes call:: "'a casino \<Rightarrow> 'a expression_monad"
-    assumes "effect (decideBet call x) s r"
-        and "inv_state pot_balance s" 
-    shows "inv r (inv_state pot_balance) (inv_state pot_balance)"
+lemma kdequals_false_dest[wpdrules]:
+assumes "kdequals a b = Some (rvalue.Value (Bool False))"
+shows "a \<noteq> b"
   using assms
-  apply (erule_tac inv_wp)
-  unfolding decideBet_def inv_state_def
-  by (vcg | auto)+
+  apply (cases a;simp add: kdequals_def)
+  apply (cases b;simp add: kdequals_def)
+  by (case_tac x4;case_tac x4a;simp add: kdequals_def split: if_split_asm)
+
+lemma kdnot_dest[wpdrules]:
+  assumes "kdnot ya = Some (rvalue.Value (Bool True))"
+  shows "ya=rvalue.Value (Bool False)"
+  using assms apply (cases ya;simp add:assms kdnot_def)
+  by (case_tac x4;simp add:assms vtnot_def)
+
+lemma vt_or_dest:
+  assumes "lift_value_binary vtor ye yg = Some (rvalue.Value (Bool True))"
+  shows "ye = rvalue.Value (Bool True) \<or> yg = rvalue.Value (Bool True)"
+ using assms
+  apply (cases ye;simp add: vtor_def)
+  apply (cases yg;simp add: vtor_def)
+  by (case_tac x4;case_tac x4a;simp)
+ 
+
+lemma kdless_dest[wpdrules]:
+  assumes "kdless (rvalue.Value (Uint x)) (rvalue.Value (Uint y)) = Some (rvalue.Value (Bool True))"
+  shows "x < y"
+ using assms
+  apply (cases x;simp add: kdless_def)
+  apply (cases y;simp add: kdless_def)
+  by (case_tac n;case_tac na;simp add: vtless_def)
+
+lemma kdequals_bool_sint[wpsimps]: "kdequals (rvalue.Value (Bool x)) (rvalue.Value (Uint y)) = None"
+  unfolding kdequals_def by simp 
 
 lemma unat_add_imp:
   assumes "(unat (x::256 word) + unat y < 115792089237316195423570985008687907853269984665640564039457584007913129639936)"
     shows "(unat (x + y) = unat x + unat y)" using assms Word.unat_add_lem[where ?'a=256, of x y] by simp
 
-lemma addToPot:
-    fixes call:: "'a casino \<Rightarrow> 'a expression_monad"
-  assumes "effect (addToPot call) s r"
-      and "inv_state pot_balance s"
-    shows "inv r (inv_state pot_balance) (inv_state pot_balance)"
-  using assms
-  apply (erule_tac inv_wp)
-  unfolding addToPot_def inv_state_def
-  by (vcg | auto dest:unat_add_imp)+
+lemma unat_mult_imp:
+  assumes "(unat (x::256 word) * unat y < 115792089237316195423570985008687907853269984665640564039457584007913129639936)"
+    shows "(unat (x * y) = unat x * unat y)" using assms Word.unat_mult_lem[where ?'a=256, of x y] by simp
 
-text \<open>
-  If a method uses a call parameter we can assume the property below and use it to discharge the first premise of @{thm wp_fallback}.
-  Then we can pass wp\_fallback to the verification condition generator using the wprule attribute.
-\<close>
+lemma unat_sub_imp:
+  assumes "(y::256 word) \<le> (x::256 word)"
+    shows "(unat (x - y) = unat x - unat y)" using assms Word.unat_sub[where ?'a=256, of y x] by simp
+
+lemma no_plus_overflow_leq:
+  assumes a:"(x ::256 word) \<le> y"
+      and b: "unat y + unat z < 2 ^ 256"
+    shows "x \<le> y + z" using no_plus_overflow_unat_size[of z y] le_no_overflow[OF a, of z]
+proof -
+  have "size z = 256" using word_size[of z] by simp
+  with b have "z \<le> z + y" using no_plus_overflow_unat_size[of z y] by simp
+  then have "x \<le> z + y" using le_no_overflow[OF a, of z] by simp
+  then show ?thesis by (simp add: add.commute)
+qed
 
 lemma 111:
+  fixes pot
   assumes "unat pot \<le> Balances s this"
       and *: "x \<le> pot"
     shows "unat (pot - x) \<le> Balances s this + unat msg_value - unat x"
  using assms unat_sub[OF *]  by simp
 
-lemma 222: "unat pot \<le> Balances s this \<Longrightarrow>
+lemma 222: "\<And>pot. unat pot \<le> Balances s this \<Longrightarrow>
        x \<le> pot \<Longrightarrow>
     unat (pot - x) \<le> Balances s this + unat msg_value"
   using 111 by fastforce
 
-lemma removeFromPot_this:
-  fixes call:: "'a casino \<Rightarrow> 'a expression_monad"
-  assumes "\<And>x. \<forall>s r. inv_state pot_balance s \<and> effect (call x) s r \<longrightarrow> local.inv r (inv_state pot_balance) (inv_state pot_balance)"
-      and "effect (removeFromPot call x) s r"
-      and "inv_state pot_balance s"
-      and "msg_sender = this"
-    shows "inv r (inv_state pot_balance) (inv_state pot_balance)"
-  using assms(2-)
-  apply (erule_tac inv_wp)
-  unfolding removeFromPot_def inv_state_def
-  by (vcg wprule: wp_fallback[OF assms(1)] | (rule 111;assumption) | (rule 222;assumption) | auto simp add:wpsimps)+
-
-lemma removeFromPot_nthis:
-  fixes call:: "'a casino \<Rightarrow> 'a expression_monad"
-  assumes "\<And>x. \<forall>s r. inv_state pot_balance s \<and> effect (call x) s r \<longrightarrow> local.inv r (inv_state pot_balance) (inv_state pot_balance)"
-      and "effect (removeFromPot call x) s r"
-      and "inv_state pot_balance s"
-      and "msg_sender \<noteq> this"
-    shows "inv r (inv_state pot_balance) (inv_state pot_balance)"
-  using assms(2-)
-  apply (erule_tac inv_wp)
-  unfolding removeFromPot_def inv_state_def
-  by (vcg wprule: wp_fallback[OF assms(1)] | (rule 111;assumption) | (rule 222;assumption) | auto simp add:wpsimps)+
-
-lemma removeFromPot:
-  fixes call:: "'a casino \<Rightarrow>'a expression_monad"
-  assumes "\<And>x. \<forall>s r. inv_state pot_balance s \<and> effect (call x) s r \<longrightarrow> local.inv r (inv_state pot_balance) (inv_state pot_balance)"
-      and "effect (removeFromPot call x) s r"
-      and "inv_state pot_balance s"
-    shows "inv r (inv_state pot_balance) (inv_state pot_balance)"
-proof (cases "msg_sender=this")
-  case True
-  then show ?thesis using removeFromPot_this[OF assms] by simp
-next
-  case False
-  then show ?thesis using removeFromPot_nthis[OF assms] by simp
-qed
-
 end
 
-invariant pot_balance: "pot_balance::(String.literal \<Rightarrow> 'a sdata) \<times> nat \<Rightarrow> bool" "pot_balance::(String.literal \<Rightarrow> 'a sdata) \<times> nat \<Rightarrow> bool" for Casino
-  apply -
-  using constructor_casino apply blast
-  using createGame apply blast
-  using placeBet apply blast
-  using decideBet apply blast
-  using addToPot apply blast
-  using removeFromPot apply blast
-  done
+method solve methods m = (m ; fail)
 
-text \<open>
-  The package then generates an overall proof over the call function:
-  @{thm Solidity.pot_balance}
-\<close>
+lemma (in Contract) wp_assign_storage111[wperules]:
+  assumes "rvalue.Value v=y"
+      and "wp (storage_update_monad [] is (K (storage_data.Value v)) i) P E s"
+    shows "wp (assign_storage i is y) P E s"
+  using assms by auto
+
+lemma notwp[wperules]: "\<not> wp m P E s \<Longrightarrow> wp m P E s \<Longrightarrow> R" using notE by simp
+
+abbreviation(in Contract) createGame_post where
+"createGame_post hN start_state return_value end_state \<equiv>
+  state.Storage end_state this STR ''state'' = storage_data.Value (Uint 1)"
+
+abbreviation(in Contract) placeBet_post where
+"placeBet_post hn start_state return_value end_state \<equiv>
+  state.Storage end_state this STR ''state'' = storage_data.Value (Uint 2)"
+
+abbreviation(in Contract) decideBet_post where
+"decideBet_post hn start_state return_value end_state \<equiv>
+  state.Storage end_state this STR ''state'' = storage_data.Value (Uint 0)"
+
+declare(in casino) pot_balanceI[wprules del]
+
+verification pot_balance:
+  pot_balance
+  createGame (\<open>K (K True)\<close>, createGame_post) and
+  placeBet (\<open>K (K True)\<close>, placeBet_post) and
+  decideBet (\<open>K (K True)\<close>, decideBet_post) and
+  addToPot and
+  removeFromPot
+  for "casino"
+proof -
+  show
+    "\<And>call.
+      (\<And>x h r. effect (call x) h r \<Longrightarrow> vcond x h r)
+      \<Longrightarrow> effect (constructor call) s r
+      \<Longrightarrow> post s r (K (K (inv_state pot_balance))) (K True)"
+    unfolding constructor_def
+    apply (erule post_exc_true, erule_tac post_wp)
+    unfolding  inv_state_def
+    by (vcg wprules: pot_balanceI | auto)+
+
+  show
+    "\<And>call hashNum.
+      (\<And>x h r. effect (call x) h r \<Longrightarrow> vcond x h r)
+      \<Longrightarrow> effect (createGame call hashNum) s r
+      \<Longrightarrow> inv_state pot_balance s
+      \<Longrightarrow> post s r (K (K (inv_state pot_balance))) (K True)"
+    unfolding createGame_def
+    apply (erule post_exc_true, erule_tac post_wp)
+    unfolding  inv_state_def
+    by (vcg wprules: pot_balanceI | solve\<open>auto simp add:wpsimps\<close>)+
+
+  show
+    "\<And>call hashNum.
+      (\<And>x h r. effect (call x) h r \<Longrightarrow> vcond x h r)
+      \<Longrightarrow> effect (createGame call hashNum) s r
+      \<Longrightarrow> inv_state pot_balance s
+      \<Longrightarrow> K (K True) hashNum s
+      \<Longrightarrow> post s r (createGame_post hashNum) (K True)"
+    unfolding createGame_def
+    apply (erule post_exc_true, erule_tac post_wp)
+    unfolding  inv_state_def
+    by (vcg wprules: pot_balanceI | solve\<open>auto simp add:wpsimps\<close>)+
+
+  show
+    "\<And>call guess.
+      (\<And>x h r. effect (call x) h r \<Longrightarrow> vcond x h r)
+      \<Longrightarrow> effect (placeBet call guess) s r
+      \<Longrightarrow> inv_state pot_balance s
+      \<Longrightarrow> post s r (K (K (inv_state pot_balance))) (K True)"
+    unfolding placeBet_def
+    apply (erule post_exc_true, erule_tac post_wp)
+    unfolding  inv_state_def
+    apply (vcg | solve\<open>auto simp add:wpsimps dest:sym\<close>)+
+                        apply (auto dest!: vt_or_dest)[1]
+                        apply (vcg wprules: pot_balanceI | solve\<open>auto simp add:wpsimps dest:sym\<close>)+
+    done
+
+  show
+    "\<And>call guess.
+      (\<And>x h r. effect (call x) h r \<Longrightarrow> vcond x h r)
+      \<Longrightarrow> effect (placeBet call guess) s r
+      \<Longrightarrow> inv_state pot_balance s
+      \<Longrightarrow> post s r (placeBet_post guess) (K True)"
+    unfolding placeBet_def
+    apply (erule post_exc_true, erule_tac post_wp)
+    unfolding inv_state_def
+    by (vcg | solve\<open>auto simp add:wpsimps dest:sym\<close>)+
+
+  show
+    "\<And>call secretNumber.
+      (\<And>x h r. effect (call x) h r \<Longrightarrow> vcond x h r)
+       \<Longrightarrow> effect (decideBet call secretNumber) s r
+       \<Longrightarrow> inv_state pot_balance s
+       \<Longrightarrow> post s r (K (K (inv_state pot_balance))) (K True)"
+    unfolding decideBet_def
+    apply (erule post_exc_true, erule_tac post_wp)
+    unfolding  inv_state_def
+    apply (vcg wprules: pot_balanceI)
+                        apply (auto simp add:wpsimps)
+                  apply (vcg wprules: pot_balanceI)
+                        apply (auto simp add:wpsimps)
+                       apply (case_tac "this = ada")
+                        apply (vcg wprules: pot_balanceI)
+                        apply (auto simp add:wpsimps dest:unat_sub_imp)
+                      apply (case_tac "this = ada")
+                       apply (vcg wprules: pot_balanceI)
+                       apply (auto simp add:wpsimps dest:sym)
+             apply (vcg wprules: pot_balanceI)
+                     apply (auto simp add:wpsimps)
+            apply (vcg wprules: pot_balanceI)
+                        apply (auto simp add:wpsimps)
+                apply (case_tac "this = ada")
+                 apply (vcg wprules: pot_balanceI)
+                 apply (auto simp add:wpsimps unat_add_imp)
+               apply (case_tac "this = ada")
+                apply (vcg wprules: pot_balanceI)
+                apply (auto simp add:wpsimps dest:sym)
+           apply (vcg wprules: pot_balanceI)
+                        apply (auto simp add:wpsimps)
+                apply (vcg wprules: pot_balanceI)
+                        apply (auto simp add:wpsimps)
+                    apply (case_tac "this = ada")
+                     apply (vcg wprules: pot_balanceI)
+                     apply (auto simp add:wpsimps dest:sym unat_sub_imp)
+            apply (vcg wprules: pot_balanceI)
+                    apply (auto simp add:wpsimps)
+           apply (vcg wprules: pot_balanceI)
+                        apply (auto simp add:wpsimps dest:sym unat_add_imp)
+          apply (vcg wprules: pot_balanceI)
+    done
+
+  show
+    "\<And>call secretNumber.
+      (\<And>x h r. effect (call x) h r \<Longrightarrow> vcond x h r)
+       \<Longrightarrow> effect (decideBet call secretNumber) s r
+       \<Longrightarrow> inv_state pot_balance s
+       \<Longrightarrow> K (K True) secretNumber s
+       \<Longrightarrow> post s r (decideBet_post secretNumber) (K True)"
+    unfolding decideBet_def
+    apply (erule post_exc_true, erule_tac post_wp)
+    unfolding inv_state_def
+    apply (vcg wprules: pot_balanceI)
+                        apply (auto simp add:wpsimps)
+                  apply (vcg wprules: pot_balanceI)
+                        apply (auto simp add:wpsimps)
+                       apply (case_tac "this = ada")
+                        apply (vcg wprules: pot_balanceI)
+                        apply (auto simp add:wpsimps dest:unat_sub_imp)
+                      apply (case_tac "this = ada")
+                       apply (vcg wprules: pot_balanceI)
+                       apply (auto simp add:wpsimps dest:sym)
+             apply (vcg wprules: pot_balanceI)
+                apply (auto simp add:wpsimps)
+             apply (case_tac "this = ada")
+              apply (vcg wprules: pot_balanceI)
+              apply (auto simp add:wpsimps dest:sym)
+           apply (vcg wprules: pot_balanceI)
+                        apply (auto simp add:wpsimps)
+                apply (vcg wprules: pot_balanceI)
+                        apply (auto simp add:wpsimps)
+                    apply (case_tac "this = ada")
+                     apply (vcg wprules: pot_balanceI)
+                     apply (auto simp add:wpsimps dest:sym unat_sub_imp)
+            apply (vcg wprules: pot_balanceI)
+               apply (auto simp add:wpsimps dest:sym unat_add_imp)
+          apply (vcg wprules: pot_balanceI)
+    done
+
+  show
+    "\<And>call.
+      (\<And>x h r. effect (call x) h r \<Longrightarrow> vcond x h r)
+      \<Longrightarrow> effect (addToPot call) s r
+      \<Longrightarrow> inv_state pot_balance s
+      \<Longrightarrow> post s r (K (K (inv_state pot_balance))) (K True)"
+    unfolding addToPot_def
+    apply (erule post_exc_true, erule_tac post_wp)
+    unfolding  inv_state_def
+    apply (vcg wprules: pot_balanceI | solve\<open>auto simp add:wpsimps dest:unat_add_imp sym\<close>)+
+                apply (auto simp add:wpsimps no_plus_overflow_leq unat_sub_imp unat_mult_imp unat_add_imp dest:sym)
+      apply (vcg wprules: pot_balanceI | solve\<open>auto simp add:wpsimps dest:unat_add_imp sym\<close>)+
+    done
+      
+  show
+    "\<And>call amount.
+      (\<And>x h r. effect (call x) h r \<Longrightarrow> vcond x h r)
+      \<Longrightarrow> effect (removeFromPot call amount) s r
+      \<Longrightarrow> inv_state pot_balance s
+      \<Longrightarrow> post s r (K (K (inv_state pot_balance))) (K True)"
+    unfolding removeFromPot_def
+    apply (erule post_exc_true, erule_tac post_wp)
+    apply (cases "msg_sender=this")
+    unfolding inv_state_def
+     apply (vcg | solve\<open>auto simp add:wpsimps dest:unat_add_imp sym\<close>)+
+         apply (drule_tac s = this in sym)
+         apply (auto simp add:wpsimps dest:unat_add_imp sym)
+         apply (vcg | solve\<open>auto simp add:wpsimps dest:unat_add_imp sym\<close>)+
+             apply (auto simp add:wpsimps dest:unat_add_imp sym)
+         apply (vcg | solve\<open>auto simp add:wpsimps dest:unat_add_imp sym\<close>)+
+               apply (auto simp add:wpsimps dest:unat_add_imp sym)
+         apply (vcg | solve\<open>auto simp add:wpsimps dest:unat_add_imp sym\<close>)+
+            apply (rule_tac pot_balanceI)
+                   apply (auto simp add:wpsimps intro: 111 222 dest:unat_add_imp sym)
+          apply (vcg | solve\<open>auto simp add:wpsimps dest:unat_add_imp sym\<close>)+
+          apply (rule_tac pot_balanceI)
+                 apply (auto simp add:wpsimps dest:unat_add_imp sym)
+         apply (vcg | solve\<open>auto simp add:wpsimps dest:unat_add_imp sym\<close>)+
+            apply (auto simp add:wpsimps dest:unat_add_imp sym)
+      apply (vcg | solve\<open>auto simp add:wpsimps dest:unat_add_imp sym\<close>)+
+            apply (auto simp add:wpsimps dest:unat_add_imp sym)
+      apply (vcg | solve\<open>auto simp add:wpsimps dest:unat_add_imp sym\<close>)+
+         apply (rule_tac pot_balanceI)
+                apply (auto simp add:wpsimps intro: 111 dest:unat_add_imp sym)
+       apply (vcg | solve\<open>auto simp add:wpsimps dest:unat_add_imp sym\<close>)+
+       apply (rule_tac pot_balanceI)
+              apply (auto simp add:wpsimps dest:unat_add_imp sym)
+      apply (vcg | solve\<open>auto simp add:wpsimps dest:unat_add_imp sym\<close>)+
+    done
+qed
+
+context casino_external
+begin
+  thm pot_balance
+  thm vcond_def
+end
 
 end
