README.md
@@ -1,1 +1,36 @@
-# isabelle-solidity-shallow
+# A Shallow Embedding of Solidity for Isabelle/HOL
+
+This directory contains a shallow embedding of Solidity in Isabelle/HOL.
+It is a copy of the corresponding [AFP entry](https://www.isa-afp.org/entries/Isabelle-Solidity.html).
+A corresponding deep embedding is available [here](https://github.com/dmarmsoler/isabelle-solidity-deep).
+
+## Prerequisites
+
+* The formalization requires [Isabelle 2025-2](https://isabelle.in.tum.de/).
+Please follow the instructions on the Isabelle home page for your operating system.
+In the following, we assume that the ``isabelle`` tool is available on the command line.
+This might require to add the Isabelle binary directory to the ``PATH`` environment variable of your system.
+
+* The formalization also requires [Finite Maps Extras](https://www.isa-afp.org/entries/Finite-Map-Extras.html) from the [AFP](https://www.isa-afp.org/).
+[Here](https://www.isa-afp.org/help/) is a guide on how to include the AFP for local builds.
+
+## Using the Formalization
+
+The formalization can be loaded into Isabelle/jEdit by executing 
+
+```sh
+isabelle jedit Solidity_Main.thy
+```
+
+on the command line. Alternatively, you can start Isabelle/jEdit by 
+clicking on the Isabelle icon and loading the theory 
+[Solidity_Main.thy](./Solidity_Main.thy) manually. 
+
+To use a command line build that also generates a PDF document,
+first add ``path/to/solidity`` to your Isabelle roots file which is
+a file called ``ROOTS`` in your Isabelle home directory.
+Then, the build can be started by executing:
+
+```sh
+isabelle build -D .
+```
